SemanticsLL.v
@@ -1,0 +1,154 @@
+(**
+
+This file describes transformations of the layout of records and arrays on
+the memory.
+
+Author: Ramon Fernandez I Mir and Arthur Charguéraud.
+
+License: MIT.
+
+*)
+
+Set Implicit Arguments.
+Require Export Typing.
+
+(* ---------------------------------------------------------------------- *)
+(** Type-directed transformation to low-level *)
+
+Inductive prefix_sum : list int -> list int -> int -> Prop :=
+  | prefix_sum_nil : forall acc,
+      prefix_sum nil nil acc
+  | prefix_sum_cons : forall l l' acc i,
+      prefix_sum l l' (i + acc) ->
+      prefix_sum (i::l) (acc::l') acc.
+
+Lemma prefix_sum_example :
+  prefix_sum (1::2::3::4::5::6::nil) (0::1::3::6::10::15::nil) 0.
+Proof.
+  repeat constructors.
+Qed.
+
+Lemma prefix_sum_length : forall l l' n,
+  prefix_sum l l' n ->
+  length l = length l'.
+Proof.
+  introv Hps. induction Hps.
+  { rewrite~ length_nil. }
+  { repeat rewrite length_cons. rewrite~ IHHps. }
+Qed.
+
+Lemma prefix_sum_spec : forall l l' n,
+  prefix_sum l l' n ->
+  (forall i,
+    index l i ->
+    l'[i] = fold_left Z.add n (take i l)).
+Proof.
+  introv Hps. induction Hps.
+  { introv Hi. false. rewrite index_eq_index_length in Hi.
+    rewrite length_nil in Hi. inverts Hi. math. }
+  { introv Hi. rewrite read_cons_case. case_if.
+    { subst. eauto. }
+    { lets Hi': Hi.
+      rewrite index_eq_index_length in Hi.
+      rewrite int_index_eq in Hi.
+      destruct Hi as (Hle&Hlt).
+      rewrite length_cons in Hlt.
+      rewrite take_cons_pos; try solve [ math ].
+      rewrite fold_left_cons.
+      asserts Hl: (index (length l) (i0 - 1)).
+      { rewrite int_index_eq. math. }
+      rewrite <- index_eq_index_length in Hl.
+      forwards*: IHHps Hl. } }
+Qed.
+
+Axiom list_to_map : forall A B, list A -> list B -> map A B.
+
+Axiom list_to_map_spec : forall ks vs m,
+  m = list_to_map ks vs ->
+      length ks = length vs
+  /\  forall i,
+        index ks i ->
+        ks[i] \indom m /\ m[ks[i]] = vs[i].
+
+Inductive ll_typdefctx_ok (C:typdefctx) (LLC:ll_typdefctx) : Prop :=
+  | low_level_ctx_ok_intros : forall CS CFOrd CFOff,
+      LLC = make_ll_typdefctx CS CFOff CFOrd ->
+      (* Same fields in C and LLC. *)
+      (forall Tv Tfs,
+        Tv \indom C ->
+        C[Tv] = typ_struct Tfs ->
+            dom Tfs = dom CFOff[Tv]
+        /\  dom Tfs = to_set CFOrd[Tv]) ->
+      (* Coherency between the sizes. *)
+      (forall Tv Tfs,
+        Tv \indom C ->
+        C[Tv] = typ_struct Tfs ->
+        (exists FT FS FO,
+            (* Fields types. *)
+            FT = List.map (fun f => Tfs[f]) CFOrd[Tv]
+            (* Fields sizes. *)
+        /\  List.Forall2 (typ_size CS) FT FS
+            (* Fields offsets. *)
+        /\  prefix_sum FS FO 0
+            (* The relationship. *)
+        /\  CS[Tv] = fold_left Z.add 0 FS
+        /\  CFOff[Tv] = list_to_map CFOrd[Tv] FO)) ->
+      ll_typdefctx_ok C LLC.
+
+(* Given a list of accesses, computes the offset. Used to translate
+   pointer values. *)
+
+Inductive tr_ll_accesses (C:typdefctx) (LLC:ll_typdefctx) : accesses -> offset -> Prop :=
+  | tr_ll_accesses_nil :
+      tr_ll_accesses C LLC nil 0%Z
+  | tr_ll_accesses_access_array : forall T T' os πs i n o,
+      typing_array C T T' os ->
+      typ_size (typvar_sizes LLC) T' n ->
+      tr_ll_accesses C LLC πs o ->
+      (0 <= i)%Z ->
+      (0 <= n)%Z ->
+      tr_ll_accesses C LLC ((access_array T i)::πs) ((i * n) + o)
+  | tr_ll_accesses_access_field : forall Tfs FO πs Tv f o,
+      typing_struct C (typ_var Tv) Tfs ->
+      FO = fields_offsets LLC ->
+      Tv \indom FO ->
+      f \indom FO[Tv] ->
+      tr_ll_accesses C LLC πs o ->
+      (0 <= FO[Tv][f])%Z ->
+      tr_ll_accesses C LLC ((access_field (typ_var Tv) f)::πs) (FO[Tv][f] + o).
+
+(* Relates values with a list of words. This is how the memory is transformed. *)
+
+Inductive tr_ll_val (C:typdefctx) (LLC:ll_typdefctx) (α:alpha) : typ -> val -> list word -> Prop :=
+  | tr_ll_val_unit :
+      tr_ll_val C LLC α typ_unit val_unit (word_int 0%Z::nil)
+  | tr_ll_val_bool : forall b,
+      tr_ll_val C LLC α typ_bool (val_bool b) (word_int (if b then 1 else 0)%Z::nil)
+  | tr_ll_val_int : forall i,
+      tr_ll_val C LLC α typ_int (val_int i) (word_int i::nil)
+  | tr_ll_val_double : forall d,
+      tr_ll_val C LLC α typ_double (val_double d) (word_int d::word_int d::nil)
+  | tr_ll_val_abstract_ptr : forall T π l o,
+      tr_ll_accesses C LLC π o ->
+      tr_ll_val C LLC α (typ_ptr T) (val_abstract_ptr l π) ((word_int (α[l] + o))::nil)
+  | tr_ll_val_array : forall k T a a',
+      length a = k ->
+      List.Forall2 (tr_ll_val C LLC α T) a a' ->
+      tr_ll_val C LLC α (typ_array T (Some k)) (val_array T a) (concat a')
+  | tr_ll_val_struct : forall FCOrd Tv Tfs sc st s s',
+      FCOrd = fields_order LLC ->
+      Tv \indom FCOrd ->
+      Tv \indom C ->
+      typing_struct C (typ_var Tv) Tfs ->
+      sc = List.map (fun f => s[f]) FCOrd[Tv] ->
+      st = List.map (fun f => Tfs[f]) FCOrd[Tv] ->
+      length s' = length FCOrd[Tv] ->
+      (forall i,
+        index s' i ->
+        tr_ll_val C LLC α st[i] sc[i] s'[i]) ->
+      tr_ll_val C LLC α (typ_var Tv) (val_struct (typ_var Tv) s) (concat s').
+
+
+(* ---------------------------------------------------------------------- *)
+(** General results about these predicates. *)
+
